Refactoring creation the Requires/Reads/Apply clauses in Boogie
Changing the types of Requires, Reads, and Apply from

[Heap, HandleType, Box, ..., Box]bool
[Heap, HandleType, Box, ..., Box]Set Box
[Heap, HandleType, Box, ..., Box]Box

to

HandleType -> [Heap, Box, ..., Box]bool
HandleType -> [Heap, Box, ..., Box]Set Box
HandleType -> [Heap, Box, ..., Box]Box

Also, factoring out the creation of the above functions into
one method rather than constructing them manually in each place.

Source/Dafny/DafnyAst.cs
@@ -4408,9 +4408,9 @@ namespace Microsoft.Dafny {
         Contract.Ensures(Contract.Result<string>() != null);
 
         if (Name == "requires") {
-          return Translator.Requires(((ArrowTypeDecl)EnclosingClass).Arity);
+          return Translator.RraName(Translator.ReqReadsApp.Requires, ((ArrowTypeDecl)EnclosingClass).Arity);
         } else if (Name == "reads") {
-          return Translator.Reads(((ArrowTypeDecl)EnclosingClass).Arity);
+          return Translator.RraName(Translator.ReqReadsApp.Reads, ((ArrowTypeDecl)EnclosingClass).Arity);
         } else {
           return EnclosingClass.FullSanitizedName + "." + CompileName;
         }
@@ -4422,9 +4422,9 @@ namespace Microsoft.Dafny {
         Contract.Ensures(Contract.Result<string>() != null);
 
         if (Name == "requires") {
-          return Translator.Requires(((ArrowTypeDecl)EnclosingClass).Arity);
+          return Translator.RraName(Translator.ReqReadsApp.Requires, ((ArrowTypeDecl)EnclosingClass).Arity);
         } else if (Name == "reads") {
-          return Translator.Reads(((ArrowTypeDecl)EnclosingClass).Arity);
+          return Translator.RraName(Translator.ReqReadsApp.Reads, ((ArrowTypeDecl)EnclosingClass).Arity);
         } else {
           return EnclosingClass.FullSanitizedRefinementName + "." + CompileName;
         }
